[lf] Various fixes in the spec due to an error in the db_init_class. Proof of the client proxy at follower done (but the problem with ghost names is to be fixed).

aneris/examples/reliable_communication/lib/repdb/spec/db_params.v
@@ -10,6 +10,7 @@ Definition Key := string.
 Class DB_params := {
   DB_addr :  socket_address;
   DB_addrF :  socket_address;
+  DB_followers : gset socket_address;
   DB_keys : gset Key;
   DB_InvName : namespace;
   DB_serialization : serialization;
